02Stack/StackConversion.thy
@@ -2,56 +2,118 @@ theory StackConversion
 imports EvaluateStack
 begin
 
-fun unfold_heap :: "nat list \<Rightarrow> expr heap \<Rightarrow> expr \<Rightarrow> expr" where
-  "unfold_heap r h e = foldr Let (map (\<lambda>x. lookup\<^sub>h x h) r) e"
+abbreviation unfold_heap :: "expr heap \<Rightarrow> expr \<Rightarrow> nat list \<Rightarrow> expr" where
+  "unfold_heap h \<equiv> foldl (\<lambda>e x. Let (lookup\<^sub>h h x) (incr\<^sub>e\<^sub>e x e))"
 
 fun unstack :: "nat list list \<Rightarrow> frame list \<Rightarrow> expr \<Rightarrow> expr heap \<Rightarrow> expr" where
-  "unstack [] s e h = undefined"
-| "unstack (r # rs) [] e h = unfold_heap r h e"
-| "unstack (r # rs) (SRef x # s) e h = unstack rs s (unfold_heap r h (Var x)) (update\<^sub>h h x e)"
-| "unstack (r # rs) (SApp e\<^sub>2 # s) e h = unstack rs s (unfold_heap r h (App e e\<^sub>2)) h"
-| "unstack (r # rs) (SProj l # s) e h = unstack rs s (unfold_heap r h (Proj e l)) h"
-| "unstack (r # rs) (SCase t cs # s) e h = unstack rs s (unfold_heap r h (Case e t cs)) h"
-| "unstack (r # rs) (SUnfold t # s) e h = unstack rs s (unfold_heap r h (Unfold t e)) h"
-| "unstack (r # rs) (STyApp t # s) e h = unstack rs s (unfold_heap r h (TyApp e t)) h"
+  "unstack [] s e h = e"
+| "unstack (r # rs) [] e h = unstack rs [] (unfold_heap h e r) h"
+| "unstack (r # rs) (SRef x # s) e h = 
+    unstack rs s (Var x) (update\<^sub>h h x (unfold_heap h e r))"
+| "unstack (r # rs) (SApp e\<^sub>2 # s) e h = unstack rs s (App (unfold_heap h e r) e\<^sub>2) h"
+| "unstack (r # rs) (SProj l # s) e h = unstack rs s (Proj (unfold_heap h e r) l) h"
+| "unstack (r # rs) (SCase t cs # s) e h = unstack rs s (Case (unfold_heap h e r) t cs) h"
+| "unstack (r # rs) (SUnfold t # s) e h = unstack rs s (Unfold t (unfold_heap h e r)) h"
+| "unstack (r # rs) (STyApp t # s) e h = unstack rs s (TyApp (unfold_heap h e r) t) h"
 
 fun unstack_state :: "nat list list \<Rightarrow> stack_state \<Rightarrow> expr" where
   "unstack_state rs (StackState (Eval e) s h) = unstack rs s e h"
 | "unstack_state rs (StackState (Return v) s h) = unstack rs s (devalue v) h"
 
-lemma tc_unstack [elim]: "\<Gamma> \<turnstile>\<^sub>s\<^sub>s s : t \<rightarrow> t' \<Longrightarrow> [],\<Gamma> \<turnstile> e : t \<Longrightarrow> h \<turnstile>\<^sub>h \<Gamma> \<Longrightarrow> 
-  distinct (concat rs) \<Longrightarrow> set (concat rs) = {x. x < length\<^sub>h h} \<Longrightarrow> length rs = Suc (length s) \<Longrightarrow>
-    [],[] \<turnstile> unstack rs s e h : t'"
-  proof (induction rs s e h rule: unstack.induct)
+abbreviation map_through :: "'a list \<Rightarrow> nat list \<Rightarrow> 'a list" where
+  "map_through \<Gamma> \<equiv> map (the o lookup \<Gamma>)"
+
+fun safe_unfold_order' :: "nat list list \<Rightarrow> nat set \<Rightarrow> expr heap \<Rightarrow> frame list \<Rightarrow> bool" where
+  "safe_unfold_order' [] xs h s = True"
+| "safe_unfold_order' ([] # rss) xs h s = safe_unfold_order' rss xs h (tl s)"
+| "safe_unfold_order' ((r # rs) # rss) xs h s = (
+    (\<forall>x. x < length\<^sub>h h \<longrightarrow> x \<notin> xs \<longrightarrow> r \<notin> free_vars (lookup\<^sub>h h x)) \<and> (r \<notin> free_vars\<^sub>s\<^sub>s s) \<and>
+      safe_unfold_order' (rs # rss) (insert r xs) h s)"
+
+fun safe_unfold_order :: "nat list list \<Rightarrow> expr heap \<Rightarrow> frame list \<Rightarrow> type list \<Rightarrow> bool" where
+  "safe_unfold_order rss h s \<Gamma> = (distinct (concat rss) \<and> length (concat rss) = length \<Gamma> \<and> h \<turnstile>\<^sub>h \<Gamma> \<and>
+    length rss = Suc (length s) \<and> (\<forall>r \<in> set (concat rss). r < length \<Gamma>) \<and> 
+      safe_unfold_order' rss {} h s)"
+
+lemma [simp]: "[],map_through \<Gamma> rs \<turnstile> e : t \<Longrightarrow> distinct rs \<Longrightarrow> h \<turnstile>\<^sub>h \<Gamma> \<Longrightarrow> length rs = length \<Gamma> \<Longrightarrow> 
+  \<forall>i < length rs. rs ! i + i < length \<Gamma> \<Longrightarrow> \<forall>x < length\<^sub>h h. \<forall>r \<in> set rs. r \<notin> free_vars (lookup\<^sub>h h x) \<Longrightarrow> 
+    unfold_heap (e, h) rs = (e', h') \<Longrightarrow> [],[] \<turnstile> e' : t"
+  proof (induction rs arbitrary: \<Gamma> e h)
+  case Nil
+    from Nil(7) have "e' = e" by simp
+    with Nil(1) show ?case by simp
+  next case (Cons r rs)
+    from Cons(2) have "[],the (lookup \<Gamma> r) # map_through (remove \<Gamma> r) rs \<turnstile> e : t" by simp
+    from Cons(3) have "distinct (r # rs)" by simp
+    from Cons(4) have "h \<turnstile>\<^sub>h \<Gamma>" by simp
+    from Cons(5) have "Suc (length rs) = length \<Gamma>" by simp
+    from Cons(6) have R: "r < length \<Gamma>" by auto
+    from Cons(6) have "\<forall>i < Suc (length rs). (r # rs) ! i + i < length \<Gamma>" by simp
+    from Cons(7) have "\<forall>x<length\<^sub>h h. \<forall>r\<in>set (r # rs). r \<notin> free_vars (lookup\<^sub>h h x)" by simp
+
+
+
+    have X: "[],map_through (remove \<Gamma> r) rs \<turnstile> lookup\<^sub>h h r : the (lookup \<Gamma> r)" by simp
+    from Cons(2) have "[],insert_at 0 (the (lookup \<Gamma> r)) (map_through (remove \<Gamma> r) rs) \<turnstile> e : t" 
+      by (cases "map_through (remove \<Gamma> r) rs") simp_all
+    with X have A: "[],map_through (remove \<Gamma> r) rs \<turnstile> Let (lookup\<^sub>h h r) e : t" by simp
+    from Cons have B: "distinct rs" by simp
+    from Cons(4, 7) R have C: "map\<^sub>h (decr\<^sub>x\<^sub>e r) (remove\<^sub>h h r) \<turnstile>\<^sub>h remove \<Gamma> r" by simp
+    from Cons(5) R have D: "length rs = length (remove \<Gamma> r)" by simp
+    from Cons(6) R have E: "\<forall>i<length rs. rs ! i + i < length (remove \<Gamma> r)" by auto
+
+
+    have F: "\<forall>x<length\<^sub>h (map\<^sub>h (decr\<^sub>x\<^sub>e r) (remove\<^sub>h h r)). \<forall>rr\<in>set rs. 
+        rr \<notin> free_vars (lookup\<^sub>h (map\<^sub>h (decr\<^sub>x\<^sub>e r) (remove\<^sub>h h r)) x)" 
+      proof (rule, rule, rule)
+        fix x rr
+        assume X: "x < length\<^sub>h (map\<^sub>h (decr\<^sub>x\<^sub>e r) (remove\<^sub>h h r))"
+
+
+        assume RS: "rr \<in> set rs"
+
+
+        from R Cons(4) have R': "r < length\<^sub>h h" by auto
+
+
+        from X R' have "incr r x < length\<^sub>h h" by (auto simp add: incr_def)
+        with Cons(7) have Y: "r \<notin> free_vars (lookup\<^sub>h h (incr r x))" by simp
+
+
+
+        have "incr r rr \<notin> free_vars (lookup\<^sub>h h (incr r x))" by simp
+        with R' Y show "rr \<notin> free_vars (lookup\<^sub>h (map\<^sub>h (decr\<^sub>x\<^sub>e r) (remove\<^sub>h h r)) x)" by simp
+      qed
+    from Cons have "unfold_heap (Let (lookup\<^sub>h h r) e, map\<^sub>h (decr\<^sub>x\<^sub>e r) (remove\<^sub>h h r)) rs = (e', h')"
+      by simp
+    with Cons(1) A B C D E F show ?case by blast
+  qed
+
+lemma tc_unstack [elim]: "map_through \<Gamma> (concat rs) \<turnstile>\<^sub>s\<^sub>s s : t \<rightarrow> t' \<Longrightarrow> 
+  [],map_through \<Gamma> (concat rs) \<turnstile> e : t \<Longrightarrow> safe_unfold_order rs h s \<Gamma> \<Longrightarrow> 
+    unstack rs s (e, h) = (e', h') \<Longrightarrow> [],[] \<turnstile> e' : t'"
+  proof (induction rs s "(e, h)" arbitrary: \<Gamma> rule: unstack.induct)
   case 1
+    thus ?case by auto
+  next case (2 rs rss \<Gamma>)
+    hence T: "t = t'" by auto
+    moreover from 2 have "[],[] \<turnstile> e' : t" by fastforce
+    ultimately show ?case by simp
+  next case (3 r rs x s eh)
     thus ?case by simp
-  next case (2 r rs e h)
-    hence "rs = []" by fastforce
-
-    from 2 have "\<Gamma> \<turnstile>\<^sub>s\<^sub>s [] : t \<rightarrow> t'" by simp
-    from 2 have "[] ,\<Gamma> \<turnstile> e : t" by simp
-    from 2 have "h \<turnstile>\<^sub>h \<Gamma>" by simp
-    from 2 have "distinct (concat (r # rs))" by simp
-    from 2 have "set (concat (r # rs)) = {x. x < length\<^sub>h h}" by simp
-
-
-    have "[],[] \<turnstile> foldr Let (map (\<lambda>x. lookup\<^sub>h x h) r) e : t'" by simp
+  next case (4 r rs e\<^sub>2 s eh)
     thus ?case by simp
-  next case 3
+  next case (5 r rs l s eh)
     thus ?case by simp
-  next case 4
+  next case (6 r rs t cs s eh)
     thus ?case by simp
-  next case 5
+  next case (7 r rs t s eh)
     thus ?case by simp
-  next case 6
-    thus ?case by simp
-  next case 7
-    thus ?case by simp
-  next case 8
+  next case (8 r rs t s eh)
     thus ?case by simp
   qed
 
-lemma tc_unstack_state [elim]: "\<Sigma> hastype t \<Longrightarrow> [],[] \<turnstile> unstack_state rs \<Sigma> : t"
+lemma tc_unstack_state [elim]: "\<Sigma> hastype t \<Longrightarrow> unstack_state rs \<Sigma> = (e, h) \<Longrightarrow> [],[] \<turnstile> e : t"
   proof (induction rs \<Sigma> rule: unstack_state.induct)
   case 1
     thus ?case using tc_unstack tc_eval_state by blast
