02Stack/TypecheckStack.thy
@@ -5,9 +5,9 @@ begin
 inductive typecheck_value :: "kind list \<Rightarrow> type list \<Rightarrow> val \<Rightarrow> type \<Rightarrow> bool" (infix ",_ \<turnstile>\<^sub>v _ :" 60) where
   tc_vabs [simp]: "\<Delta>,insert_at 0 t\<^sub>1 \<Gamma> \<turnstile> e : t\<^sub>2 \<Longrightarrow> \<Delta> \<turnstile>\<^sub>k t\<^sub>1 : Star \<Longrightarrow> \<Delta>,\<Gamma> \<turnstile>\<^sub>v VAbs t\<^sub>1 e : Arrow t\<^sub>1 t\<^sub>2"
 | tc_vrec [simp]: "\<Delta>,\<Gamma> \<turnstile>\<^sub>x\<^sub>s fs : ts \<Longrightarrow> \<Delta>,\<Gamma> \<turnstile>\<^sub>v VRec fs : Record ts"
-| tc_vinj [simp]: "lookup x \<Gamma> = Some t \<Longrightarrow> lookup l ts = Some t \<Longrightarrow> \<forall>tt \<in> set ts. \<Delta> \<turnstile>\<^sub>k tt : Star \<Longrightarrow> 
+| tc_vinj [simp]: "lookup \<Gamma> x = Some t \<Longrightarrow> lookup ts l = Some t \<Longrightarrow> \<forall>tt \<in> set ts. \<Delta> \<turnstile>\<^sub>k tt : Star \<Longrightarrow> 
     \<Delta>,\<Gamma> \<turnstile>\<^sub>v VInj l ts x : Variant ts"
-| tc_vfold [simp]: "lookup x \<Gamma> = Some (subst\<^sub>t\<^sub>t 0 (Inductive k t) t) \<Longrightarrow> 
+| tc_vfold [simp]: "lookup \<Gamma> x = Some (subst\<^sub>t\<^sub>t 0 (Inductive k t) t) \<Longrightarrow> 
     insert_at 0 k \<Delta> \<turnstile>\<^sub>k t : Star \<Longrightarrow> \<Delta>,\<Gamma> \<turnstile>\<^sub>v VFold t x : Inductive k t"
 | tc_vtyabs [simp]: "insert_at 0 k \<Delta>,map (incr\<^sub>t\<^sub>t 0) \<Gamma> \<turnstile> e : t \<Longrightarrow> \<Delta>,\<Gamma> \<turnstile>\<^sub>v VTyAbs k e : Forall k t"
 
@@ -18,9 +18,9 @@ inductive_cases [elim]: "\<Delta>,\<Gamma> \<turnstile>\<^sub>v VFold t' e : t"
 inductive_cases [elim]: "\<Delta>,\<Gamma> \<turnstile>\<^sub>v VTyAbs k e : t"
 
 inductive typecheck_frame :: "type list \<Rightarrow> frame \<Rightarrow> type \<Rightarrow> type \<Rightarrow> bool" (infix "\<turnstile>\<^sub>s _ : _ \<rightarrow>" 60) where
-  tc_sref [simp]: "lookup x \<Gamma> = Some t \<Longrightarrow> \<Gamma> \<turnstile>\<^sub>s SRef x : t \<rightarrow> t"
+  tc_sref [simp]: "lookup \<Gamma> x = Some t \<Longrightarrow> \<Gamma> \<turnstile>\<^sub>s SRef x : t \<rightarrow> t"
 | tc_sapp [simp]: "[],\<Gamma> \<turnstile> e : t' \<Longrightarrow> \<Gamma> \<turnstile>\<^sub>s SApp e : Arrow t' t \<rightarrow> t"
-| tc_sproj [simp]: "lookup l ts = Some t \<Longrightarrow> \<Gamma> \<turnstile>\<^sub>s SProj l : Record ts \<rightarrow> t"
+| tc_sproj [simp]: "lookup ts l = Some t \<Longrightarrow> \<Gamma> \<turnstile>\<^sub>s SProj l : Record ts \<rightarrow> t"
 | tc_scase [simp]: "[],\<Gamma> \<turnstile>\<^sub>c cs : ts \<rightarrow> t \<Longrightarrow> \<Gamma> \<turnstile>\<^sub>s SCase t cs : Variant ts \<rightarrow> t"
 | tc_sunfold [simp]: "[k] \<turnstile>\<^sub>k t : Star \<Longrightarrow> 
     \<Gamma> \<turnstile>\<^sub>s SUnfold t : Inductive k t \<rightarrow> subst\<^sub>t\<^sub>t 0 (Inductive k t) t"
@@ -42,7 +42,7 @@ inductive_cases [elim]: "\<Gamma> \<turnstile>\<^sub>s\<^sub>s [] : t \<rightarr
 inductive_cases [elim]: "\<Gamma> \<turnstile>\<^sub>s\<^sub>s f # s : t \<rightarrow> t'"
 
 inductive typecheck_heap :: "expr heap \<Rightarrow> type list \<Rightarrow> bool" (infix "\<turnstile>\<^sub>h" 60) where
-  tch_heap [simp]: "(\<And>i t. lookup i \<Gamma> = Some t \<Longrightarrow> [],\<Gamma> \<turnstile> lookup\<^sub>h i h : t) \<Longrightarrow> 
+  tch_heap [simp]: "(\<And>i t. lookup \<Gamma> i = Some t \<Longrightarrow> [],\<Gamma> \<turnstile> lookup\<^sub>h h i : t) \<Longrightarrow> 
     length\<^sub>h h = length \<Gamma> \<Longrightarrow> h \<turnstile>\<^sub>h \<Gamma>"
 
 inductive_cases [elim]: "h \<turnstile>\<^sub>h \<Gamma>"
@@ -58,17 +58,17 @@ inductive_cases [elim]: "StackState (Return v) s h hastype t"
 
 lemma tc_devalue [simp]: "\<Delta>,\<Gamma> \<turnstile>\<^sub>v v : t \<Longrightarrow> \<Delta>,\<Gamma> \<turnstile> devalue v : t"
   proof (induction \<Delta> \<Gamma> v t rule: typecheck_value.inducts)
-  case (tc_vinj x \<Gamma> t l ts \<Delta>)
-    hence "lookup x \<Gamma> = Some t" by simp
-    moreover from tc_vinj have "lookup l ts = Some t" by simp
+  case (tc_vinj \<Gamma> x t ts l \<Delta>)
+    hence "lookup \<Gamma> x = Some t" by simp
+    moreover from tc_vinj have "lookup ts l = Some t" by simp
     moreover from tc_vinj have "\<forall>tt \<in> set ts. \<Delta> \<turnstile>\<^sub>k tt : Star" by simp
     ultimately show ?case by simp
   qed simp_all
 
-lemma [simp]: "h \<turnstile>\<^sub>h \<Gamma> \<Longrightarrow> lookup x \<Gamma> = Some t \<Longrightarrow> [],\<Gamma> \<turnstile> e : t \<Longrightarrow> update\<^sub>h h x e \<turnstile>\<^sub>h \<Gamma>"
+lemma [simp]: "h \<turnstile>\<^sub>h \<Gamma> \<Longrightarrow> lookup \<Gamma> x = Some t \<Longrightarrow> [],\<Gamma> \<turnstile> e : t \<Longrightarrow> update\<^sub>h h x e \<turnstile>\<^sub>h \<Gamma>"
   proof (induction h \<Gamma> rule: typecheck_heap.induct)
   case (tch_heap \<Gamma> h)
-    hence "\<And>i t. lookup i \<Gamma> = Some t \<Longrightarrow> [],\<Gamma> \<turnstile> lookup\<^sub>h i (update\<^sub>h h x e) : t" by auto
+    hence "\<And>i t. lookup \<Gamma> i = Some t \<Longrightarrow> [],\<Gamma> \<turnstile> lookup\<^sub>h (update\<^sub>h h x e) i : t" by auto
     moreover from tch_heap have "length\<^sub>h (update\<^sub>h h x e) = length \<Gamma>" by simp
     ultimately show ?case by (metis typecheck_heap.tch_heap)
   qed
@@ -76,8 +76,8 @@ lemma [simp]: "h \<turnstile>\<^sub>h \<Gamma> \<Longrightarrow> lookup x \<Gamm
 lemma [simp]: "h \<turnstile>\<^sub>h \<Gamma> \<Longrightarrow> [],\<Gamma> \<turnstile> e : t \<Longrightarrow> extend\<^sub>h h e \<turnstile>\<^sub>h insert_at (length\<^sub>h h) t \<Gamma>"
   proof (induction h \<Gamma> rule: typecheck_heap.induct)
   case (tch_heap \<Gamma> h)
-    moreover hence "\<And>i tt. lookup i (insert_at (length\<^sub>h h) t \<Gamma>) = Some tt \<Longrightarrow> 
-        [],insert_at (length\<^sub>h h) t \<Gamma> \<turnstile> lookup\<^sub>h i (extend\<^sub>h h e) : tt"
+    moreover hence "\<And>i tt. lookup (insert_at (length\<^sub>h h) t \<Gamma>) i = Some tt \<Longrightarrow> 
+        [],insert_at (length\<^sub>h h) t \<Gamma> \<turnstile> lookup\<^sub>h (extend\<^sub>h h e) i : tt"
       using lookup_less_than by fastforce
     ultimately show ?case by simp
   qed
@@ -98,5 +98,22 @@ lemma tc_stack_weaken [simp]: "\<Gamma> \<turnstile>\<^sub>s\<^sub>s s : t \<rig
     moreover from tcs_cons have "insert_at (length \<Gamma>) tt \<Gamma> \<turnstile>\<^sub>s f : t \<rightarrow> t'" by simp
     ultimately show ?case by simp
   qed simp_all
+
+lemma [simp]: "h \<turnstile>\<^sub>h \<Gamma> \<Longrightarrow> r < length \<Gamma> \<Longrightarrow> \<forall>i < length\<^sub>h h. r \<notin> free_vars (lookup\<^sub>h h i) \<Longrightarrow> 
+    map\<^sub>h (decr\<^sub>x\<^sub>e r) (remove\<^sub>h h r) \<turnstile>\<^sub>h remove \<Gamma> r"
+  proof (induction h \<Gamma> rule: typecheck_heap.induct) 
+  case (tch_heap \<Gamma> h)
+    have "\<And>i t. lookup (remove \<Gamma> r) i = Some t \<Longrightarrow> 
+        [],remove \<Gamma> r \<turnstile> lookup\<^sub>h (map\<^sub>h (decr\<^sub>x\<^sub>e r) (remove\<^sub>h h r)) i : t"
+      proof -
+        fix i t
+        assume I: "lookup (remove \<Gamma> r) i = Some t" 
+        with tch_heap have "incr r i < length\<^sub>h h" by auto
+        with tch_heap I show "[],remove \<Gamma> r \<turnstile> lookup\<^sub>h (map\<^sub>h (decr\<^sub>x\<^sub>e r) (remove\<^sub>h h r)) i : t" by simp
+      qed
+    moreover from tch_heap have "length\<^sub>h (map\<^sub>h (decr\<^sub>x\<^sub>e r) (remove\<^sub>h h r)) = length (remove \<Gamma> r)" 
+      by simp
+    ultimately show ?case by simp
+  qed
 
 end
