Utilities/Heap.thy
@@ -1,5 +1,5 @@
 theory Heap
-imports Main
+imports Index
 begin
 
 datatype 'a heap = Heap "nat \<Rightarrow> 'a" nat
@@ -10,14 +10,20 @@ definition empty\<^sub>h :: "'a heap" where
 primrec length\<^sub>h :: "'a heap \<Rightarrow> nat" where
   "length\<^sub>h (Heap h n) = n"
 
-primrec lookup\<^sub>h :: "nat \<Rightarrow> 'a heap \<Rightarrow>'a" where
-  "lookup\<^sub>h x (Heap h n) = h x"
+primrec lookup\<^sub>h :: "'a heap \<Rightarrow>nat \<Rightarrow> 'a" where
+  "lookup\<^sub>h (Heap h n) x = h x"
 
 primrec extend\<^sub>h :: "'a heap \<Rightarrow> 'a \<Rightarrow> 'a heap" where
   "extend\<^sub>h (Heap h n) a = Heap (h(n := a)) (Suc n)"
 
 primrec update\<^sub>h :: "'a heap \<Rightarrow> nat \<Rightarrow> 'a \<Rightarrow> 'a heap" where
   "update\<^sub>h (Heap h n) x a = Heap (h(x := a)) n"
+
+primrec remove\<^sub>h :: "'a heap \<Rightarrow> nat \<Rightarrow> 'a heap" where
+  "remove\<^sub>h (Heap h n) x = Heap (h o incr x) (n - 1)"
+
+primrec map\<^sub>h :: "('a \<Rightarrow> 'b) \<Rightarrow> 'a heap \<Rightarrow> 'b heap" where
+  "map\<^sub>h f (Heap h n) = Heap (f o h) n"
 
 lemma [simp]: "length\<^sub>h empty\<^sub>h = 0"
   by (simp add: empty\<^sub>h_def)
@@ -28,10 +34,22 @@ lemma [simp]: "length\<^sub>h (extend\<^sub>h h a) = Suc (length\<^sub>h h)"
 lemma length\<^sub>h_update\<^sub>h [simp]: "length\<^sub>h (update\<^sub>h h x a) = length\<^sub>h h"
   by (induction h) simp_all
 
-lemma [simp]: "lookup\<^sub>h y (update\<^sub>h h x a) = (if x = y then a else lookup\<^sub>h y h)"
+lemma [simp]: "x < length\<^sub>h h \<Longrightarrow> length\<^sub>h (remove\<^sub>h h x) = length\<^sub>h h - 1"
   by (induction h) simp_all
 
-lemma [simp]: "lookup\<^sub>h x (extend\<^sub>h h a) = (if x = length\<^sub>h h then a else lookup\<^sub>h x h)"
+lemma [simp]: "length\<^sub>h (map\<^sub>h f h) = length\<^sub>h h"
+  by (induction h) simp_all
+
+lemma [simp]: "lookup\<^sub>h (update\<^sub>h h x a) y = (if x = y then a else lookup\<^sub>h h y)"
+  by (induction h) simp_all
+
+lemma [simp]: "lookup\<^sub>h (extend\<^sub>h h a) x = (if x = length\<^sub>h h then a else lookup\<^sub>h h x)"
+  by (induction h) simp_all
+
+lemma [simp]: "x < length\<^sub>h h \<Longrightarrow> lookup\<^sub>h (remove\<^sub>h h x) y = lookup\<^sub>h h (incr x y)"
+  by (induction h) simp_all
+
+lemma [simp]: "lookup\<^sub>h (map\<^sub>h f h) x = f (lookup\<^sub>h h x)"
   by (induction h) simp_all
 
 end
