Utilities/Vector.thy
@@ -8,13 +8,21 @@ fun insert_at :: "nat \<Rightarrow> 'a \<Rightarrow> 'a list \<Rightarrow> 'a li
 | "insert_at (Suc x) a' [] = undefined"
 | "insert_at (Suc x) a' (a # as) = a # insert_at x a' as"
 
-fun lookup :: "nat \<Rightarrow> 'a list \<Rightarrow> 'a option" where
-  "lookup x [] = None"
-| "lookup 0 (a # as) = Some a"
-| "lookup (Suc x) (a # as) = lookup x as"
+fun lookup :: "'a list \<Rightarrow> nat \<Rightarrow> 'a option" where
+  "lookup [] x = None"
+| "lookup (a # as) 0 = Some a"
+| "lookup (a # as) (Suc x) = lookup as x"
+
+fun remove :: "'a list \<Rightarrow> nat \<Rightarrow> 'a list" where
+  "remove [] x = undefined"
+| "remove (a # as) 0 = as"
+| "remove (a # as) (Suc x) = a # remove as x"
 
 lemma insert_length [simp]: "x \<le> length as \<Longrightarrow> length (insert_at x a as) = Suc (length as)"
   by (induction x a as rule: insert_at.induct) simp_all
+
+lemma [simp]: "x < length as \<Longrightarrow> length (remove as x) = length as - 1"
+  by (induction as x rule: remove.induct) simp_all
 
 lemma [simp]: "x \<le> length as \<Longrightarrow> y \<le> x \<Longrightarrow> 
     insert_at y b (insert_at x a as) = insert_at (Suc x) a (insert_at y b as)"
@@ -23,23 +31,36 @@ lemma [simp]: "x \<le> length as \<Longrightarrow> y \<le> x \<Longrightarrow>
     thus ?case by (induction y) simp_all
   qed simp_all
 
-lemma [simp]: "x \<le> length as \<Longrightarrow> lookup x (insert_at x a as) = Some a"
+lemma [simp]: "x < length as \<Longrightarrow> y \<le> x \<Longrightarrow> 
+    insert_at y a (remove as x) = remove (insert_at y a as) (Suc x)"
+  proof (induction as x arbitrary: y rule: remove.induct)
+  case (2 a as)
+    thus ?case 
+      proof (induction y)
+      case 0
+        thus ?case by (induction as) simp_all
+      qed simp_all
+  next case 3
+    thus ?case by (induction y) simp_all
+  qed simp_all
+
+lemma [simp]: "x \<le> length as \<Longrightarrow> lookup (insert_at x a as) x = Some a"
   by (induction x a as rule: insert_at.induct) simp_all
 
-lemma [simp]: "lookup x as = Some a \<Longrightarrow> lookup x (insert_at (length as) a' as) = Some a"
-  by (induction x as rule: lookup.induct) simp_all
+lemma [simp]: "lookup as x = Some a \<Longrightarrow> lookup (insert_at (length as) a' as) x = Some a"
+  by (induction as x rule: lookup.induct) simp_all
 
-lemma [elim]: "lookup x (insert_at (length as) a' as) = Some a \<Longrightarrow> x < length as \<Longrightarrow> 
-    lookup x as = Some a"
-  by (induction x as rule: lookup.induct) fastforce+
+lemma [elim]: "lookup (insert_at (length as) a' as) x = Some a \<Longrightarrow> x < length as \<Longrightarrow> 
+    lookup as x = Some a"
+  by (induction as x rule: lookup.induct) fastforce+
 
-lemma [simp]: "x \<le> length as \<Longrightarrow> y < x \<Longrightarrow> lookup y (insert_at x a as) = lookup y as"
+lemma [simp]: "x \<le> length as \<Longrightarrow> y < x \<Longrightarrow> lookup (insert_at x a as) y = lookup as y"
   proof (induction x a as arbitrary: y rule: insert_at.induct)
   case 4
     thus ?case by (induction y) simp_all
   qed simp_all
 
-lemma [simp]: "x \<le> length as \<Longrightarrow> x \<le> y \<Longrightarrow> lookup (Suc y) (insert_at x a as) = lookup y as"
+lemma [simp]: "x \<le> length as \<Longrightarrow> x \<le> y \<Longrightarrow> lookup (insert_at x a as) (Suc y) = lookup as y"
   proof (induction x a as arbitrary: y rule: insert_at.induct)
   case 4
     thus ?case by (induction y) simp_all
@@ -48,20 +69,23 @@ lemma [simp]: "x \<le> length as \<Longrightarrow> x \<le> y \<Longrightarrow> l
 lemma [simp]: "x \<le> length as \<Longrightarrow> map f (insert_at x a as) = insert_at x (f a) (map f as)"
   by (induction x a as rule: insert_at.induct) simp_all
 
-lemma [simp]: "lookup x (map f as) = map_option f (lookup x as)"
-  by (induction x as rule: lookup.induct) simp_all
+lemma [simp]: "x < length as \<Longrightarrow> map f (remove as x) = remove (map f as) x"
+  by (induction as x rule: remove.induct) simp_all
 
-lemma lookup_less_than [elim]: "lookup x as = Some a \<Longrightarrow> x < length as"
-  by (induction x as rule: lookup.induct) simp_all
+lemma [simp]: "lookup (map f as) x = map_option f (lookup as x)"
+  by (induction as x rule: lookup.induct) simp_all
 
-lemma [elim]: "list_all p as \<Longrightarrow> lookup x as = Some a \<Longrightarrow> p a"
-  by (induction x as rule: lookup.induct) simp_all
+lemma lookup_less_than [elim]: "lookup as x = Some a \<Longrightarrow> x < length as"
+  by (induction as x rule: lookup.induct) simp_all
 
-lemma [simp]: "x < length as \<Longrightarrow> lookup x (as @ bs) = lookup x as"
-  by (induction x as rule: lookup.induct) simp_all
+lemma [elim]: "list_all p as \<Longrightarrow> lookup as x = Some a \<Longrightarrow> p a"
+  by (induction as x rule: lookup.induct) simp_all
 
-lemma [simp]: "lookup (length as + x) (as @ bs) = lookup x bs"
-  by (induction "length as + x" as rule: lookup.induct) simp_all
+lemma [simp]: "x < length as \<Longrightarrow> lookup (as @ bs) x = lookup as x"
+  by (induction as x rule: lookup.induct) simp_all
+
+lemma [simp]: "lookup (as @ bs) (length as + x) = lookup bs x"
+  by (induction as "length as + x" rule: lookup.induct) simp_all
 
 lemma [simp]: "x \<le> length as \<Longrightarrow> insert_at x a (as @ bs) = insert_at x a as @ bs"
   by (induction x a as rule: insert_at.induct) (cases bs, simp_all)
