Utilities/Misc.thy
@@ -1,0 +1,14 @@
+theory Misc
+imports Main
+begin
+
+primrec map_fst :: "('a \<Rightarrow> 'c) \<Rightarrow> 'a \<times> 'b \<Rightarrow> 'c \<times> 'b" where
+  "map_fst f (a, b) = (f a, b)"
+
+lemma [simp]: "(x::nat) \<ge> y \<Longrightarrow> \<exists>z. x = y + z"
+  proof (induction x arbitrary: y)
+  case Suc
+    thus ?case by (induction y) simp_all
+  qed simp_all
+
+end
